rewrite: hope i got things right this time

srv.v
@@ -7,20 +7,20 @@ From iris.algebra Require Import upred frac excl dec_agree upred_big_op gset gma
 From iris.tests Require Import atomic treiber_stack.
 From flatcomb Require Import misc.
 
-Definition doOp : val :=
-  λ: "f" "p",
+Definition doOp (f: val) : val :=
+  λ: "p",
      match: !"p" with
-       InjL "x" => "p" <- InjR ("f" "x")
+       InjL "x" => "p" <- InjR (f "x")
      | InjR "_" => #()
      end.
 
-Definition loop : val :=
-  rec: "loop" "p" "f" "s" "lk" :=
+Definition loop (f: val): val :=
+  rec: "loop" "p" "s" "lk" :=
     match: !"p" with
       InjL "_" =>
         if: CAS "lk" #false #true
-          then iter (doOp "f") "s"
-          else "loop" "p" "f" "s" "lk"
+          then iter (doOp f) "s"
+          else "loop" "p" "s" "lk"
     | InjR "r" => "r"
     end.
 
@@ -31,240 +31,127 @@ Definition install : val :=
      push "s" "p";;
      "p".
 
-Definition flat : val :=
+Definition flat (f: val) : val :=
   λ: "f",
      let: "lk" := ref (#false) in
      let: "s" := new_stack #() in
      λ: "x",
         let: "p" := install "x" "s" in
-        loop "p" "f" "s" "lk".
+        loop f "p" "s" "lk".
 
 Global Opaque doOp install loop flat.
 
 Definition srvR := prodR fracR (dec_agreeR val).
-Class srvG Σ := SrvG { srv_G :> inG Σ srvR }.
-Definition srvΣ : gFunctors := #[GFunctor (constRF srvR)].
+Definition tokR := evmapR loc (gname * gname * gname * gname).
+Class srvG Σ := SrvG {
+  srv_G :> inG Σ srvR;
+  tok_G :> inG Σ (authR tokR);
+}.
+
+Definition srvΣ : gFunctors :=
+  #[ GFunctor (constRF srvR);
+     GFunctor (constRF (authR tokR))
+   ].
+
 Instance subG_srvΣ {Σ} : subG srvΣ Σ → srvG Σ.
-Proof. intros [?%subG_inG _]%subG_inv. split; apply _. Qed.
+Proof. intros [?%subG_inG [?%subG_inG _]%subG_inv]%subG_inv. split; apply _. Qed.
 
 Section proof.
   Context `{!heapG Σ, !lockG Σ, !evidenceG loc val Σ, !srvG Σ} (N : namespace).
 
   Definition p_inv
-             (γx γ1 γ2 γ3 γ4: gname)
+             (γm γx γ1 γ2 γ3 γ4: gname)
              (Q: val → val → Prop)
              (v: val): iProp Σ :=
-    ((∃ (y: val), v = InjRV y ★ own γ1 (Excl ()) ★ own γ3 (Excl ())) ∨
-     (∃ (x: val), v = InjLV x ★ own γx ((1/2)%Qp, DecAgree x) ★ own γ1 (Excl ()) ★ own γ4 (Excl ())) ∨
-     (∃ (x: val), v = InjLV x ★ own γx ((1/4)%Qp, DecAgree x) ★ own γ2 (Excl ()) ★ own γ4 (Excl ())) ∨
-     (∃ (x y: val), v = InjRV y ★ own γx ((1/2)%Qp, DecAgree x) ★ ■ Q x y ★ own γ1 (Excl ()) ★ own γ4 (Excl ())))%I.
+    (∃ (p : loc) (q: Qp), v = #p ★ own γm (◯ ({[ p := (q, DecAgree (γx, γ1, γ3, γ4)) ]} : tokR)) ★
+     ((∃ (y: val), p ↦ InjRV y ★ own γ1 (Excl ()) ★ own γ3 (Excl ())) ∨
+      (∃ (x: val), p ↦ InjLV x ★ own γx ((1/2)%Qp, DecAgree x) ★ own γ1 (Excl ()) ★ own γ4 (Excl ())) ∨
+      (∃ (x: val), p ↦ InjLV x ★ own γx ((1/4)%Qp, DecAgree x) ★ own γ2 (Excl ()) ★ own γ4 (Excl ())) ∨
+      (∃ (x y: val), p ↦ InjRV y ★ own γx ((1/2)%Qp, DecAgree x) ★ ■ Q x y ★ own γ1 (Excl ()) ★ own γ4 (Excl ()))))%I.
 
-  Definition p_inv_R γ2 Q v : iProp Σ := (∃ γx γ1 γ3 γ4: gname, p_inv γx γ1 γ2 γ3 γ4 Q v)%I.
+  Definition p_inv_R γm γ2 Q v : iProp Σ :=
+    (∃ γx γ1 γ3 γ4: gname, p_inv γm γx γ1 γ2 γ3 γ4 Q v)%I.
 
-  Definition srv_inv (γ γ2: gname) (s: loc) (Q: val → val → Prop) : iProp Σ :=
-    (∃ xs, is_stack' (p_inv_R γ2 Q) xs s γ)%I.
+  Definition srv_stack_inv (γ γm γ2: gname) (s: loc) (Q: val → val → Prop) : iProp Σ :=
+    (∃ xs, is_stack' (p_inv_R γm γ2 Q) xs s γ)%I.
 
-  Instance p_inv_timeless γx γ1 γ2 γ3 γ4 p Q: TimelessP (p_inv γx γ1 γ2 γ3 γ4 p Q).
-  Proof. apply _. Qed.
+  Definition srv_m_inv γm := (∃ m, own γm (● m))%I.
 
-  Instance srv_inv_timeless γ γ2 s Q: TimelessP (srv_inv γ γ2 s Q).
+  Lemma install_push_spec
+        (Φ: val → iProp Σ) (Q: val → val → Prop)
+        (p: loc) (γ γm γx γ1 γ2 γ3 γ4: gname)
+        (s: loc) (x: val) :
+    heapN ⊥ N →
+    heap_ctx ★ inv N (srv_stack_inv γ γm γ2 s Q) ★ own γx ((1/2)%Qp, DecAgree x) ★
+    own γm (◯ ({[ p := ((1 / 2)%Qp, DecAgree (γx, γ1, γ3, γ4)) ]})) ★
+    p ↦ InjLV x ★ own γ1 (Excl ()) ★ own γ4 (Excl ()) ★ (True -★ Φ #())
+    ⊢ WP push #s #p {{ Φ }}.
   Proof.
-    apply uPred.exist_timeless.
-    move=>x. apply is_stack'_timeless.
-    move=>v. apply _.
+    iIntros (HN) "(#Hh & #? & Hx & Hpm & Hp & Ho1 & Ho2 & HΦ)".
+    rewrite /srv_stack_inv.
+    iDestruct (push_spec N (p_inv_R γm γ2 Q) with "[-HΦ]") as "Hpush"=>//.
+    - iFrame "Hh". iSplitL "Hx Hp Hpm Ho1 Ho2"; last eauto.
+      iExists γx, γ1, γ3, γ4. iExists p, (1/2)%Qp. iSplit=>//. iFrame "Hpm".
+      iRight. iLeft.
+      iExists x. iFrame.
+    - iApply wp_wand_r.
+      iSplitL "Hpush"; first done.
+      iIntros (?). iIntros "%".
+      inversion H. by iApply "HΦ".
   Qed.
 
-  (* Lemma push_spec *)
-  (*       (Φ: val → iProp Σ) (Q: val → val → Prop) *)
-  (*       (p: loc) (γx γ1 γ2 γ3 γ4: gname) *)
-  (*       (γhd γgn: gname) (s: loc) (x: val) : *)
-  (*   heapN ⊥ N → *)
-  (*   heap_ctx ★ inv N (srv_inv γhd γgn s Q) ★ own γx ((1/2)%Qp, DecAgree x) ★ *)
-  (*   p ↦ InjLV x ★ own γ1 (Excl ()) ★ own γ4 (Excl ()) ★ (True -★ Φ #()) *)
-  (*   ⊢ WP push #s #p {{ Φ }}. *)
-  (* Proof. *)
-  (*   iIntros (HN) "(#Hh & #Hsrv & Hp & Hx & Ho1 & Ho4 & HΦ)".     *)
-  (*   iDestruct (push_atomic_spec N s #p with "Hh") as "Hpush"=>//. *)
-  (*   rewrite /push_triple /atomic_triple. *)
-  (*   iSpecialize ("Hpush" $! (p ↦ InjLV x ★ own γ1 (Excl ()) ★ own γ4 (Excl ()) ★ *)
-  (*                            own γx ((1/2)%Qp, DecAgree x))%I *)
-  (*                           (fun _ ret => ret = #())%I with "[]"). *)
-  (*   - iIntros "!#". iIntros "(Hp & Hx & Ho1 & Ho4)". *)
-  (*     (* open the invariant *) *)
-  (*     iInv N as (hds gnm) ">(Hohd & Hogn & Hxs & Hhd & Hps)" "Hclose". *)
-  (*     iDestruct "Hxs" as (xs) "(Hs & Hgn)". *)
-  (*     (* mask magic *) *)
-  (*     iApply pvs_intro'. *)
-  (*     { apply ndisj_subseteq_difference; auto. } *)
-  (*     iIntros "Hvs". *)
-  (*     iExists (map (λ x : loc, #x) xs). *)
-  (*     iFrame "Hs". iSplit. *)
-  (*     + (* provide a way to rollback *) *)
-  (*       iIntros "Hl'". *)
-  (*       iVs "Hvs". iVs ("Hclose" with "[-Hp Hx Ho1 Ho4]"); last by iFrame. *)
-  (*       iNext. rewrite /srv_inv. iExists hds, gnm. *)
-  (*       iFrame. iExists xs. by iFrame. *)
-  (*     + (* provide a way to commit *) *)
-  (*       iIntros (?) "[% Hs]". subst. *)
-  (*       iVs "Hvs". iVs ("Hclose" with "[-]"); last done. *)
-  (*       iNext. rewrite /srv_inv. iExists hds, (gnm ∪ {[ p := DecAgree (γx, γ1, γ2, γ3, γ4) ]}). *)
-  (*       iFrame. *)
-  (*       iClear "Hogn". *)
-  (*       iAssert (own γgn (● (gnm ∪ {[p := DecAgree (γx, γ1, γ2, γ3, γ4)]})) ★ *)
-  (*                own γgn (◯ {[ p := DecAgree (γx, γ1, γ2, γ3, γ4) ]}))%I as "[Hogn' Hfrag]". *)
-  (*       { admit. } *)
-  (*       iFrame. iSplitL "Hs Hgn". *)
-  (*       { iExists (p::xs). *)
-  (*         iFrame. admit. } *)
-  (*       iSplitL "Hhd". *)
-  (*       { admit. } *)
-  (*       iAssert (p_inv' (DecAgree (γx, γ1, γ2, γ3, γ4)) p Q)  with "[Hp Hx Ho1 Ho4]" as "Hinvp". *)
-  (*       { rewrite /p_inv' /p_inv. iRight. iLeft. iExists x. by iFrame. } *)
-  (*       admit. *)
-  (*   - iApply wp_wand_r. iSplitR "HΦ". *)
-  (*     + iApply "Hpush". by iFrame. *)
-  (*     + iIntros (?) "H". iDestruct "H" as (?) "%". subst. by iApply "HΦ". *)
-  (* Admitted. *)
-
-  (* Lemma install_spec *)
-  (*       (Φ: val → iProp Σ) (Q: val → val → Prop) *)
-  (*       (x: val) (γhd γgn: gname) (s: loc): *)
-  (*   heapN ⊥ N → *)
-  (*   heap_ctx ★ inv N (srv_inv γhd γgn s Q) ★ *)
-  (*   (∀ (p: loc) (γx γ1 γ2 γ3 γ4: gname), *)
-  (*      own γ2 (Excl ()) -★ own γ3 (Excl ()) -★ own γgn (◯ {[ p := DecAgree (γx, γ1, γ2, γ3, γ4) ]}) -★ *)
-  (*      own γx ((1/2)%Qp, DecAgree x) -★ Φ #p) *)
-  (*   ⊢ WP install x #s {{ Φ }}. *)
-  (* Proof. *)
-  (*   iIntros (HN) "(#Hh & #Hsrv & HΦ)". *)
-  (*   wp_seq. wp_let. wp_alloc p as "Hl". *)
-  (*   iVs (own_alloc (Excl ())) as (γ1) "Ho1"; first done. *)
-  (*   iVs (own_alloc (Excl ())) as (γ2) "Ho2"; first done. *)
-  (*   iVs (own_alloc (Excl ())) as (γ3) "Ho3"; first done. *)
-  (*   iVs (own_alloc (Excl ())) as (γ4) "Ho4"; first done. *)
-  (*   iVs (own_alloc (1%Qp, DecAgree x)) as (γx) "Hx"; first done. *)
-  (*   iDestruct (own_update with "Hx") as "==>[Hx1 Hx2]". *)
-  (*   { by apply pair_l_frac_op_1'. } *)
-  (*   wp_let. wp_bind ((push _) _). *)
-  (*   iApply push_spec=>//. *)
-  (*   iFrame "Hh Hsrv Hx1 Hl Ho1 Ho4". *)
-  (*   iIntros "_". wp_seq. iVsIntro. *)
-  (*   iSpecialize ("HΦ" $! p γx γ1 γ2 γ3 γ4). *)
-  (*   iAssert (own γgn (◯ {[p := DecAgree (γx, γ1, γ2, γ3, γ4)]})) as "Hfrag". *)
-  (*   { admit. } *)
-  (*   iApply ("HΦ" with "Ho2 Ho3 Hfrag Hx2"). *)
-  (* Admitted. *)
-
-  (* Definition pinv_sub RI γx γ1 γ2 γ3 γ4 p Q := (RI ⊣⊢ ∃ Rf, Rf ★ p_inv γx γ1 γ2 γ3 γ4 p Q)%I. *)
-
-  (* Lemma doOp_spec Φ (f: val) (RI: iProp Σ) γx γ1 γ2 γ3 γ4 p Q `{TimelessP _ RI}: *)
-  (*   heapN ⊥ N → pinv_sub RI γx γ1 γ2 γ3 γ4 p Q → *)
-  (*   heap_ctx ★ inv N RI ★ own γ2 (Excl ()) ★ *)
-  (*   □ (∀ x:val, WP f x {{ v, ■ Q x v }})%I ★ (own γ2 (Excl ()) -★ Φ #()) *)
-  (*   ⊢ WP doOp f #p {{ Φ }}. *)
-  (* Proof. *)
-  (*   iIntros (HN Hsub) "(#Hh & #HRI & Ho2 & #Hf & HΦ)". *)
-  (*   wp_seq. wp_let. wp_bind (! _)%E. *)
-  (*   iInv N as ">H" "Hclose". *)
-  (*   iDestruct (Hsub with "H") as (Rf) "[HRf [Hp | [Hp | [Hp | Hp]]]]". *)
-  (*   - iDestruct "Hp" as (y) "(Hp & Ho1 & Ho3)". *)
-  (*     wp_load. iVs ("Hclose" with "[HRf Hp Ho1 Ho3]"). *)
-  (*     { iNext. iApply Hsub. iExists Rf. iFrame "HRf". *)
-  (*       iLeft. iExists y. by iFrame. } *)
-  (*     iVsIntro. wp_match. by iApply "HΦ". *)
-  (*   - iDestruct "Hp" as (x) "(Hp & Hx & Ho1 & Ho4)". *)
-  (*     wp_load. *)
-  (*     iAssert (|=r=> own γx (((1 / 4)%Qp, DecAgree x) ⋅ ((1 / 4)%Qp, DecAgree x)))%I with "[Hx]" as "==>[Hx1 Hx2]". *)
-  (*     { iDestruct (own_update with "Hx") as "Hx"; last by iAssumption. *)
-  (*       replace ((1 / 2)%Qp) with (1/4 + 1/4)%Qp; last by apply Qp_div_S. *)
-  (*       by apply pair_l_frac_op'. } *)
-  (*     iVs ("Hclose" with "[HRf Hp Hx1 Ho2 Ho4]"). *)
-  (*     { iNext. iApply Hsub. iExists Rf. iFrame "HRf". *)
-  (*       iRight. iRight. iLeft. iExists x. by iFrame. } *)
-  (*     iVsIntro. wp_match. *)
-  (*     wp_bind (f _). iApply wp_wand_r. *)
-  (*     iSplitR; first by iApply "Hf". *)
-  (*     iIntros (y) "%". *)
-  (*     iInv N as ">H" "Hclose". *)
-  (*     iDestruct (Hsub with "H") as (Rf') "[HRf [Hp | [Hp | [Hp | Hp]]]]". *)
-  (*     + admit. *)
-  (*     + admit. *)
-  (*     + iDestruct "Hp" as (x') "(Hp & Hx & Ho2 & Ho4)". *)
-  (*       destruct (decide (x = x')) as [->|Hneq]; last by admit. *)
-  (*       iCombine "Hx2" "Hx" as "Hx". *)
-  (*       iDestruct (own_update with "Hx") as "==>Hx"; first by apply pair_l_frac_op. *)
-  (*       rewrite Qp_div_S. *)
-  (*       wp_store. iVs ("Hclose" with "[HRf Hp Hx Ho1 Ho4]"). *)
-  (*       { iNext. iApply Hsub. iExists Rf'. iFrame "HRf". *)
-  (*         iRight. iRight. iRight. iExists x', y. *)
-  (*         by iFrame. } *)
-  (*       iVsIntro. by iApply "HΦ". *)
-  (*     + admit. *)
-  (*   - admit. *)
-  (*   - admit. *)
-  (* Admitted. *)
-
-  Lemma loop_iter_list_spec Φ (f: val) (s hd: loc) Q (γhd γgn γ2: gname) xs:
+  Lemma install_spec
+        (Φ: val → iProp Σ) (Q: val → val → Prop)
+        (x: val) (γ2 γm γ: gname) (s: loc):
     heapN ⊥ N →
-    heap_ctx ★ inv N (srv_inv γhd γgn γ2 s Q) ★ □ (∀ x:val, WP f x {{ v, ■ Q x v }})%I ★ own γ2 (Excl ()) ★
-    is_list hd xs ★ own γhd (◯ ({[ hd ]} : hdsetR)) ★ (own γ2 (Excl ()) -★ Φ #())
-    ⊢ WP doOp f {{ f', WP iter' #hd f' {{ Φ  }} }}.
+    heap_ctx ★ inv N (srv_stack_inv γ γm γ2 s Q) ★ inv N (srv_m_inv γm) ★ 
+    (∀ (p: loc) (γx γ1 γ2 γ3 γ4: gname),
+       own γ3 (Excl ()) -★ own γm (◯ {[ p := ((1 / 2)%Qp, DecAgree (γx, γ1, γ3, γ4)) ]}) -★
+       own γx ((1/2)%Qp, DecAgree x) -★ Φ #p)
+    ⊢ WP install x #s {{ Φ }}.
   Proof.
-    iIntros (HN) "(#Hh & #? & #Hf & Hxs & Hhd & Ho2 & HΦ)".
-    rewrite /doOp. wp_let.
-    iLöb as "IH".
-    wp_rec. wp_let. wp_bind (! _)%E.
-    destruct xs as [|x xs'].
-    - simpl. iDestruct "Hhd" as (q) "Hhd".
-      wp_load. wp_match. by iApply "HΦ".
-    - simpl. iDestruct "Hhd" as (hd' q) "[[Hhd1 Hhd2] Hhd']".
-      wp_load. wp_match. wp_proj. wp_let.
-      wp_bind (! _)%E.
-      iInv N as (hds gnm) ">(Hohd & Hogn & Hxse & Hhds & Hps)" "Hclose".
-      iAssert (∃ (p: loc) γs, x = #p ★ p_inv' γ2 γs p Q)%I as "Hx".
-      { admit. }
-      iDestruct "Hx" as (p γs) "[% Hp]". subst.
-      rewrite /p_inv'. destruct γs as [[[[γx γ1] γ3] γ4]|].
-      iDestruct "Hp" as "[Hp | [Hp | [ Hp | Hp]]]"=>//.
-      + admit.
-      + iDestruct "Hp" as (x) "(Hp & Hx & Ho1 & Ho4)".
-        iAssert (|=r=> own γx (((1 / 4)%Qp, DecAgree x) ⋅ ((1 / 4)%Qp, DecAgree x)))%I with "[Hx]" as "==>[Hx1 Hx2]".
-        { iDestruct (own_update with "Hx") as "Hx"; last by iAssumption.
-          replace ((1 / 2)%Qp) with (1/4 + 1/4)%Qp; last by apply Qp_div_S.
-          by apply pair_l_frac_op'. }
-        wp_load. iVs ("Hclose" with "[-Ho1 Hx2 Hhd2 HΦ]").
-        { iNext. iExists hds, gnm. by iFrame. }
-        iVsIntro. wp_match.
-        wp_bind (f _). iApply wp_wand_r. iSplitR; first by iApply "Hf".
-        iIntros (y) "Q". 
-        iInv N as (hds' gnm') ">(Hohd & Hogn & Hxse & Hhds & Hps)" "Hclose".
-        iAssert (p_inv' γ2 (DecAgree (γx, γ1, γ3, γ4)) p Q)%I as "Hp".
-        { admit. }
-        rewrite /p_inv'.
-        iDestruct "Hp" as "[Hp | [Hp | [ Hp | Hp]]]".
-        * admit.
-        * admit.
-        * iDestruct "Hp" as (x') "(Hp & Hx' & Ho2 & Ho4)".
-          destruct (decide (x = x')) as [->|Hneq]; last by admit.
-          iCombine "Hx2" "Hx'" as "Hx".
-          iDestruct (own_update with "Hx") as "==>Hx"; first by apply pair_l_frac_op.
-          rewrite Qp_div_S.
-          wp_store. iVs ("Hclose" with "[-Ho2 HΦ Hhd2]").
-          { iNext. iExists hds', gnm'. by iFrame. }
-          iVsIntro. wp_seq. wp_proj. rewrite /doOp.
-          iAssert (is_list hd' xs') as "Hl".
-          { admit. }
-          iAssert (∃ (hd'0 : loc) (q0 : Qp),
-                     hd ↦{q0} SOMEV (#p, #hd'0) ★ is_list hd'0 xs')%I with "[Hhd2 Hl]" as "He".
-          { iExists hd', (q / 2)%Qp. by iFrame. }
-          iAssert (own γhd (◯ {[hd]})) as "Hfrag".
-          { admit. }
-          iSpecialize ("IH" with "Ho2 He Hfrag HΦ").
-          admit.
-        * admit.
-      + admit.
-      + admit.
-      + by iExFalso.
+    iIntros (HN) "(#Hh & #? & #? & HΦ)".
+    wp_seq. wp_let. wp_alloc p as "Hl".
+    iVs (own_alloc (Excl ())) as (γ1) "Ho1"; first done.
+    iVs (own_alloc (Excl ())) as (γ3) "Ho3"; first done.
+    iVs (own_alloc (Excl ())) as (γ4) "Ho4"; first done.
+    iVs (own_alloc (1%Qp, DecAgree x)) as (γx) "Hx"; first done.
+    iDestruct (own_update with "Hx") as "==>[Hx1 Hx2]"; first by apply pair_l_frac_op_1'.
+    wp_let. wp_bind ((push _) _).
+    iApply install_push_spec=>//.
+    iFrame "#".
+    iAssert (own γm (◯ {[p := ((1/2)%Qp, DecAgree (γx, γ1, γ3, γ4))]} ⋅
+                     ◯ {[p := ((1/2)%Qp, DecAgree (γx, γ1, γ3, γ4))]})) as "[Hfrag1 Hfrag2]".
+    { admit. }
+    iFrame "Hx1 Hfrag1 Hl Ho1 Ho4". iIntros "_". wp_seq. iVsIntro.
+    iSpecialize ("HΦ" $! p γx γ1 γ2 γ3 γ4 with "[-Hx2 Hfrag2]")=>//.
+    iApply ("HΦ" with "Hfrag2 Hx2").
+  Admitted.
+
+  Lemma loop_iter_list_spec Φ (f: val) (s hd: loc) Q (γ γm γ2: gname) xs:
+    heapN ⊥ N →
+    heap_ctx ★ inv N (srv_stack_inv γ γm γ2 s Q) ★ □ (∀ x:val, WP f x {{ v, ■ Q x v }})%I ★ own γ2 (Excl ()) ★
+    is_list' γ hd xs ★ (own γ2 (Excl ()) -★ Φ #())
+    ⊢ WP iter' #hd (doOp f) {{ Φ }}.
+  Proof.
+    iIntros (HN) "(#Hh & #? & #Hf & Ho2 & Hlist' & HΦ)".
+    rewrite /doOp.
+    iApply pvs_wp.
+    iDestruct (dup_is_list' with "[Hlist']") as "==>[Hl1 Hl2]"; first by iFrame.
+    iDestruct (dup_is_list' with "[Hl2]") as "==>[Hl2 Hl3]"; first by iFrame.
+    iDestruct (iter'_spec _ (p_inv_R γm γ2 Q) _ γ s (is_list' γ hd xs ★ own γ2 (Excl ()))%I xs hd (λ: "p",
+      match: ! "p" with InjL "x" => "p" <- SOME (f "x") | InjR "_" => #() end)%V (λ: "p",
+      match: ! "p" with InjL "x" => "p" <- SOME (f "x") | InjR "_" => #() end) with "[-Hl1]") as "Hiter'"=>//.
+    - rewrite /f_spec.
+      iIntros (Φ' x _ Hin) "(#Hh & #? & (Hls & Ho2) & HΦ')".
+      wp_let. wp_bind (! _)%E. iInv N as (xs') ">Hs" "Hclose".
+      iDestruct "Hs" as (hd') "[Hhd [Hxs HRs]]".
+      (* now I know x conforms to p_inv_R *)
+      admit.
+    - apply to_of_val.
+    - iFrame "#". iFrame "Hl2 Hl3 Ho2".
+      iIntros "[_ H]". by iApply "HΦ".
+    - done.
   Admitted.
 
   Lemma loop_iter_spec Φ (f: val) (s: loc) Q (γhd γgn γ2: gname):
